Improving structure of m0_progTheary

playground/uart_model/.hollogs/m0u_progTheory.sig
@@ -1,0 +1,45 @@
+Specializing fetch: 2 -> 2(2)
+Specializing decode Thumb: 82 -> 82(82)
+Specializing decode Thumb-2: 1 -> 1(1)
+Specializing decode Thumb (fallback): 1 -> 1(1)
+Specializing decode Thumb-2 (fallback): 1 -> 1(1)
+Specializing eval: 72 -> 72(72)
+Specializing eval: 72 -> 72(72)
+<<HOL message: Created theory "m0u_prog">>
+Saved theorem _____ "datatype_m0u_component"
+Saved theorem _____ "m0u_component_11"
+Saved theorem _____ "m0u_component_distinct"
+Saved theorem _____ "m0u_component_nchotomy"
+Saved theorem _____ "m0u_component_Axiom"
+Saved theorem _____ "m0u_component_induction"
+Saved theorem _____ "m0u_component_case_cong"
+Saved theorem _____ "m0u_component_case_eq"
+<<HOL message: Defined type: "m0u_component">>
+Saved theorem _____ "datatype_m0u_data"
+Saved theorem _____ "m0u_data_11"
+Saved theorem _____ "m0u_data_distinct"
+Saved theorem _____ "m0u_data_nchotomy"
+Saved theorem _____ "m0u_data_Axiom"
+Saved theorem _____ "m0u_data_induction"
+Saved theorem _____ "m0u_data_case_cong"
+Saved theorem _____ "m0u_data_case_eq"
+<<HOL message: Defined type: "m0u_data">>
+<<HOL message: mk_functional: The following input rows (counting from zero) are inaccessible: 4, 5, 6.
+They have been ignored.>>
+Saved definition __ "m0u_proj_def"
+Saved definition __ "TO_M0U_def"
+Saved definition __ "TO_M0U_PROP_def"
+Saved definition __ "r2m0_c_set_def"
+Saved definition __ "UART_def"
+Saved definition __ "DOM_def"
+Saved theorem _____ "m0_SDOM_STAR_thm"
+Saved definition __ "NextStateM0U_def"
+Saved definition __ "M0U_MODEL_def"
+Saved definition __ "COSIM_def"
+Saved theorem _____ "NEX_thm"
+Saved theorem _____ "NIT_NIT_STEP_thm"
+error in quse /home/daniil/projects/Kvasir/playground/uart_model/m0u_progScript.sml : Fail "Static Errors"
+error in load m0u_progScript : Fail "Static Errors"
+Saved theorem _____ "NIT_COSIM_thm"
+/home/daniil/projects/Kvasir/playground/uart_model/m0u_progScript.sml:297: error: ; expected but val was found
+Uncaught exception: Fail "Static Errors"
