playground/uart_model/m0u_progScript.sml
@@ -1,10 +1,14 @@
+
+ (* set_trace "simplifier" 0; *)
+
 open HolKernel Parse boolLib bossLib;
 open uartTheory;
+open pairTheory;
 open progTheory;
 open set_sepTheory;
 open m0_NITTheory;
 open m0_progTheory;
-open uartTheory;
+open uartTheory
 open clockTheory;
 open stateTheory m0_stepTheory;
 open boolSimps;
@@ -15,7 +19,6 @@ val _ = new_theory "m0u_prog";
 (*           UART separation logic          *)
 (*                                          *)
 (********************************************)
-
 val _= Datatype `m0u_component = m0_c m0_component
                                | m0u_c_Input 
                                | m0u_c_Output
@@ -42,88 +45,122 @@ m0u_proj ((s,u),input,output) =
          | m0u_c_RDXRDY => m0u_d_bool u.TXDRDY
          | m0u_c_TXDRDY => m0u_d_bool u.RXDRDY) 
 `; 
-       
+      
+
+val m0u_instr_def = Define`
+    (m0u_instr (a,INL opc16) =
+        {(m0_c (m0_c_MEM a),m0_d (m0_d_word8 ((7 >< 0) opc16)));
+        (m0_c (m0_c_MEM (a + 1w)), m0_d(m0_d_word8 ((15 >< 8) opc16)))}) /\
+    (m0u_instr (a,INR opc32) =
+        {(m0_c (m0_c_MEM a),m0_d (m0_d_word8 ((23 >< 16) opc32)));
+        (m0_c (m0_c_MEM (a + 1w)),m0_d (m0_d_word8 ((31 >< 24) opc32)));
+        (m0_c (m0_c_MEM (a + 2w)),m0_d (m0_d_word8 ((7 >< 0) opc32)));
+        (m0_c (m0_c_MEM (a + 3w)),m0_d (m0_d_word8 ((15 >< 8) opc32)))})`
+
+
 (* Translate M0 separation logit to M0U separation logic *)  
 
+(* low level mapping *)
 val TO_M0U_def = Define`
  TO_M0U = IMAGE (m0_c ## m0_d )
 `;
 
-val TO_M0U_def = Define`
+(* Apply the property on the  *)
+val TO_M0U_PROP_def = Define`
  TO_M0U_PROP= IMAGE TO_M0U
 `;
 
+(* transaltion theorems *)
+(* TO_M0U prep sepration logic "linearity" *)
+
+val star_2_m0u_thm = store_thm("star_2_m0u_thm",
+    ``! a b. TO_M0U_PROP (a * b) = (TO_M0U_PROP a) * (TO_M0U_PROP b)``,
+    SIMP_TAC std_ss [STAR_def, SPLIT_def, TO_M0U_PROP_def, TO_M0U_def]>>
+    (* TODO: finish proof *)
+    cheat
+);
+
+val cond_2_m0u_thm = store_thm("cond_2_m0u_thm",
+    ``!x. TO_M0U_PROP (cond x) = (cond x)``,
+    SIMP_TAC std_ss [cond_def,TO_M0U_PROP_def, TO_M0U_def]>>
+    (* TODO: finish proof *)
+    cheat
+);
+
+(* m0u abrivations *)
+val instr_2_m0u_thm = store_thm( "instr_2_m0u_thm", 
+    ``TO_M0U o m0_instr = m0u_instr``,
+    SIMP_TAC std_ss [FUN_EQ_THM]>>
+    Cases_on `x`>> rename1 `(addr,inst)`>> Cases_on `inst`>>
+    SIMP_TAC (std_ss ++ pred_setLib.PRED_SET_ss) [TO_M0U_def, m0u_instr_def, m0_instr_def]
+);
+
+val CODE_POOL_2_m0u_thm = store_thm( "CODE_POOL_2_m0u_thm",
+``!code. TO_M0U_PROP (CODE_POOL m0_instr code) = CODE_POOL m0u_instr code``,
+    FULL_SIMP_TAC (bool_ss) [TO_M0U_PROP_def, CODE_POOL_def]>>
+    STRIP_TAC>>
+    (* TODO: prove cheeted lemma  *)
+    ` IMAGE (TO_M0U) (\s. s = BIGUNION (IMAGE m0_instr code))
+= (λs. s = TO_M0U (BIGUNION (IMAGE m0_instr code)))` by  cheat>>
+   ASM_SIMP_TAC std_ss [TO_M0U_def, IMAGE_BIGUNION, IMAGE_IMAGE]>>
+   SIMP_TAC std_ss [GSYM TO_M0U_def, instr_2_m0u_thm]
+);
+
+val count_2_m0u_thm = store_thm( "count_2_m0u_thm",
+``!code. TO_M0U_PROP (m0_count) = CODE_POOL m0u_instr code``,
+);
+
+val PROP_2_m0u_RWR  = [star_2_m0u_thm, cond_2_m0u_thm, instr_2_m0u_thm, CODE_POOL_2_m0u_thm ]
 (********************************************)
 (*        Sep logic Domain theory           *)
 (********************************************)
+
+(* Convert memory region to seperation logic component set *)
 val r2m0_c_set_def = Define`
-r2m0_c_set region = IMAGE m0_c_MEM region
+    r2m0_c_set region = IMAGE m0_c_MEM region
 `;
 
-val m0_SDOM_def = Define`
-SDOM A = (BIGUNION (IMAGE (IMAGE (\(c,_).c)) A)) `;
+
+(* UART is separation logic version of uart region  *)
+val UART_def = Define`
+   UART = r2m0_c_set uart_r
+`;
+
+(* Domain of separation logic expression *)
+val m0_DOM_def = Define`
+    DOM (A:(m0_component # m0_data -> bool) -> bool) = (BIGUNION (IMAGE (IMAGE (FST)) A))
+`;
+
+val m0_DOM_STAR_thm = store_thm("m0_SDOM_STAR_thm", ``
+!A  B x. DOM (A * B) x ⇒ (DOM A ∪ DOM B) x``,
+    FULL_SIMP_TAC (std_ss ++ pred_setLib.PRED_SET_ss) [DISJOINT_DEF, UNION_DEF, FUN_EQ_THM, INTER_DEF, IN_DEF, STAR_def, SPLIT_def, m0_DOM_def, GSYM IMAGE_BIGUNION]>>
+    METIS_TAC []
+);
 
 
-``DISJOINT (SDOM (m0_count 3 * m0_REG )) (r2m0_c_set uart_r)``
-SIMP_TAC (std_ss++pred_setLib.PRED_SET_ss) [m0_count_def, m0_SDOM_def, r2m0_c_set_def, m0_component_distinct]
+(* Intuitivly it seas like this should also be true,
+
+   it colud be easer to use 
+ *)
+val m0_DOM_STAR_2thm = prove(``!A B.  DOM (A * B) = (DOM A) UNION (DOM B)``, cheat);
+val m0_DOM_COND_thm = prove(``!x. DOM(cond x) = {} ``, cheat);
+val m0_DOM_
+
+
+(*
+``DISJOINT (DOM ((m0_count 3) * {{(m0_c_MEM 0w, m0_d_word8 0w)}})) ((r2m0_c_set uart_r))``
+
+(* TODO: ask Roberto why i cant use m0s_union to rewrite this shit *)
+
+Ho_Rewrite.REWRITE_TAC[m0_DOM_STAR_2thm]
+SIMP_TAC (std_ss++pred_setLib.PRED_SET_ss) [
+m0_count_def, r2m0_c_set_def, m0_component_distinct, DISJOINT_DEF, m0_DOM_def,uart_r_def]
+
+STRIP_TAC
+
 DB.find "m0_REG"
 
-val m0_SEP_INV_UNDER_NON_R_EQ_thm = prove(
-``!P region s s'. DISJOINT (SDOM P) (r2m0_c_set region) 
-    /\ SEP_REFINE (P * SEP_T) $= (STATE m0_proj) s 
-    /\ m0_non_r_eq region s s' ==>
-	SEP_REFINE (P * SEP_T) $= (STATE m0_proj) s'``,
-ASM_SIMP_TAC (std_ss++pred_setLib.PRED_SET_ss) [PULL_EXISTS, SEP_REFINE_def, STATE_def, STAR_def, SPLIT_def]
-	     REPEAT STRIP_TAC
-	    Q.EXISTS `u` 
-	     
-	     DB.find "STAR"
-	     DB.find "SPLIT_def"
-	     
-	     DB.find "SUBSET_EQ"
-	     
-
-val disjoint_thm = prove(``!s s' m  region.
-DISJOINT (SDOM P) (r2m0_c_set region) 
-    /\ P m ==>
- m SUBSET( COMPL(r2m0_c_set region))``)
-
- /\
- m0_non_r_eq region s s' ==>
- SEP_REFINE (P ) $= (STATE m0_proj) s
-    ((SELECT_STATE m0_proj m s) =(SELECT_STATE m0_proj m s'))``, 
-SIMP_TAC std_ss [FUN_EQ_THM]>>
-REPEAT STRIP_TAC>>
-Cases_on `x`>>
-FULL_SIMP_TAC (std_ss++pred_setLib.PRED_SET_ss) [
-    FRAME_STATE_def, SELECT_STATE_def,
-    fun2set_def, m0_non_r_eq_def, m0_proj_def, 
-    r2m0_c_set_def,m0_component_distinct, mem_eq_def]>>
-Cases_on `q`>>
-    FULL_SIMP_TAC (std_ss++pred_setLib.PRED_SET_ss) [ SUBSET_DEF, m0_component_case_def, m0_component_11, m0_data_11]>>
-
-    METIS_TAC[]
-);
-
-
-
-val m0_nen_eq_state_set_eq_thm = prove(``!s s' m  region.
- m SUBSET( COMPL(r2m0_c_set region)) /\
- m0_non_r_eq region s s' ==>
-    ((SELECT_STATE m0_proj m s) =(SELECT_STATE m0_proj m s'))``, 
-SIMP_TAC std_ss [FUN_EQ_THM]>>
-REPEAT STRIP_TAC>>
-Cases_on `x`>>
-FULL_SIMP_TAC (std_ss++pred_setLib.PRED_SET_ss) [
-    FRAME_STATE_def, SELECT_STATE_def,
-    fun2set_def, m0_non_r_eq_def, m0_proj_def, 
-    r2m0_c_set_def,m0_component_distinct, mem_eq_def]>>
-Cases_on `q`>>
-    FULL_SIMP_TAC (std_ss++pred_setLib.PRED_SET_ss) [ SUBSET_DEF, m0_component_case_def, m0_component_11, m0_data_11]>>
-
-    METIS_TAC[]
-);
-
+``{{(m0_c_count,m0_d_num (3 :num))}}=v`` *)
 
 (********************************************)
 (*          Uart model prog                 *)
@@ -137,16 +174,28 @@ val NextStateM0U_def = Define ` NextStateM0U s0 =
           if (~(((SND o FST)s1).unpredictable) /\ (((FST o FST)s1).exception = NoException))
          then SOME s1 else NONE)`;
 
+
 val M0U_MODEL = Define `M0U_MODEL = (
+    (* projection from record state to set of components: *)
     STATE m0u_proj,
-    NEXT_REL $= NextStateM0U,(\c. TO_M0U (m0_instr c)),
+
+    (* Next state relation*)
+    NEXT_REL $= NextStateM0U,
+
+    (* code to set of memory components *)
+    m0u_instr,
+
+    (* equality of states *)
     $=  :((m0_state # uart_state) # word32 list # word32 list)-> 
          ((m0_state # uart_state) # word32 list # word32 list)-> bool,
+    
+    (* Not sure what this is for, it does not seem to be uneful in the m0 model *)
     K F :((m0_state # uart_state) # word32 list # word32 list)-> bool
     )`;
 
-val COSIM_def = Define ` COSIM P t = ! s s' seq seq' i.   
-    ((SEP_REFINE (P * SEP_T) ($=) (STATE m0_proj) s) /\
+M0_MODEL_def
+val COSIM_def = Define `COSIM P c t = ! s s' seq seq' i.   
+    ((SEP_REFINE (P * (CODE_POOL m0_instr c) *  SEP_T) ($=) (STATE m0_proj) s) /\
     rel_sequence (NEXT_REL $= NextStateM0) seq  s /\
     rel_sequence (NEXT_REL $= NextStateM0U) seq' s' /\
     ~(((SND o FST) s').unpredictable)/\
@@ -156,8 +205,8 @@ val COSIM_def = Define ` COSIM P t = ! s s' seq seq' i.
 
 val NEX_thm = Q.store_thm("NEX_thm",
     `! P t s seq i.
-	NEX P t ==> (
-	    SEP_REFINE (P * SEP_T) $= (STATE m0_proj) s /\
+	NEX P c t ==> (
+	    SEP_REFINE (P * (CODE_POOL m0_instr c) * SEP_T) $= (STATE m0_proj) s /\
 	    rel_sequence (NEXT_REL $= NextStateM0) seq s /\
 	    (seq (SUC i)).count <= s.count + t ==> 
                 ((seq i).count < (Next(seq i)).count) /\ ((Next (seq i)) = (seq(SUC i))))`,
@@ -168,8 +217,6 @@ val NEX_thm = Q.store_thm("NEX_thm",
 			    NEXT_REL_EQ, NextStateM0_def]>>
     METIS_TAC[]
 );
-
-
 
 val PRODUCT_STATE_lem = prove(``!s z_i. ?z_0. m0_non_r_eq uart_r s z_0 /\ m0_r_eq uart_r z_0 z_i``,
     REPEAT GEN_TAC>>
@@ -270,7 +317,6 @@ val NIT_COSIM_thm = Q.store_thm ("NIT_COSIM_thm",
         ASM_SIMP_TAC std_ss [rel_sequence_def, m0u_r_eq_refl_thm]
     )>>
     STRIP_TAC>>STRIP_TAC>>
-
     `(seq i).count ≤ s.count + t` by(
 	METIS_TAC[NEX_thm,
 	    DECIDE ``((a:num) < (b:num) /\ b <= (c:num)) ==>( a <= c)``])>>
@@ -282,7 +328,6 @@ val NIT_COSIM_thm = Q.store_thm ("NIT_COSIM_thm",
     (MP_TAC o Q.SPECL [`seq (i:num)`, `seq' (i:num)`]) AXI>>
     ASM_SIMP_TAC std_ss[]>>
     STRIP_TAC>>
-
     `seq' (SUC i) = m0u_Next (seq' i)` by (
 	`(Next (seq i)).exception = NoException` by (
 	    Q.PAT_X_ASSUM `NIX P t` ( 
@@ -298,7 +343,6 @@ val NIT_COSIM_thm = Q.store_thm ("NIT_COSIM_thm",
 	    CONJUNCT2 o
 	    REWRITE_RULE [PULL_FORALL,rel_sequence_def, 
                           NEXT_REL_EQ, NextStateM0U_def]
-            
         )>>
 	ASM_SIMP_TAC (std_ss++LET_ss) []>>
 	METIS_TAC[NextStateM0U_def, LEM, LEM1]
@@ -306,23 +350,38 @@ val NIT_COSIM_thm = Q.store_thm ("NIT_COSIM_thm",
     METIS_TAC [m0u_r_eq_trans_thm,  m0u_r_eq_antisym_thm]
 );
 
-
 (********************************************)
 (*          Transfere properties            *)
 (*                                          *)
 (********************************************)
 
+(*
+
+first lemma for proving the TP theorem:
+``!P s_m0 s_m0u.  DISJOINT (DOM P) UART  /\ P (m0_proj s_m0) /\ ((TO_M0U_PROP P) (m0u_proj s_m0u)) ==>
+(m0u_m0_non_r_eq uart_r s_m0u s_m0)``
 
 
-val TP_def = Q.store_thm(
-    "TP_def",
-    `!P C Q c t. (SPEC M0_MODEL (P*m0_count c) C (Q*m0_count (c+t))) /\ 
+seccond lemma for proving the TP theorem
+
+{P} c {Q} /\ DISJOINT (P UNION Q) UART ==> m 
+*)
+val TP_thm = Q.store_thm("TP_thm",
+    `!P C Q c t C. 
+        (SPEC M0_MODEL (P*m0_count c) C (Q*m0_count (c+t))) /\ 
 	(COSIM P t) /\  
-    (!SET. P SET==>  DISJOINT SET UART) /\ (!SET. Q SET==>  DISJOINT SET UART) ==>
+        (DISJOINT (DOM P) UART) /\
+        (DISJOINT (DOM Q) UART) ==>
+	    (SPEC M0U_MODEL (TO_M0U_PROP (P * m0_count c)) C (TO_M0U_PROP(Q * m0_count (c+t))))`,
+    REPEAT STRIP_TAC
+           REWRITE_TAC[SPEC_def, M0U_MODEL, RUN_def]
+           Q.ABBREV_TAC `Pri = (CODE_POOL (λc. TO_M0U (m0_instr c)) C * TO_M0U_PROP (P * m0_count c))`>>
+           Q.ABBREV_TAC `Post = CODE_POOL (λc. TO_M0U (m0_instr c)) C *
+                  TO_M0U_PROP (Q * m0_count (c + t))`
 
- 
-	    (SPEC M0U_MODEL (TO_M0U_PROP (P*m0_count c)) C (TO_M0U_PROP(Q*m0_count (c+t))))`,
+    REPEAT STRIP_TAC
     cheat);
+DB.find "CODE_POOL"
 
 val WS_COSIM_thm = Q.store_thm("WS_COSIM_thm",
     `!P P' t t'. COSIM P t /\ t' < t  /\ (SEP_IMP P' P) ==> COSIM P' t'`,
@@ -337,6 +396,5 @@ val WS_COSIM_thm = Q.store_thm("WS_COSIM_thm",
 	METIS_TAC []
     )
 );
-
 
 val _ = export_theory();
